bit-vector interpretation using Bedrock words.
-TODO (complete the admitted proofs):
-- prove that CVC4 multiplication is equivalent to word multiplication
-- prove that CVC4 signed comparison is equivalent to word signed comparison

src/Trace.v
@@ -291,9 +291,13 @@ Module Cnf_Checker.
 
  Lemma checker_b_correct : forall t_var t_form l b c,
     checker_b t_form l b c = true ->
-    Lit.interp (Form.interp_state_var (PArray.get t_var) (fun _ s => BITVECTOR_LIST.zeros s) t_form) l = b.
+    Lit.interp (Form.interp_state_var (PArray.get t_var) (fun _ s => Word.wzero s) t_form) l = b.
  Proof.
-   unfold checker_b; intros t_var t_form l b c; case b; case_eq (Lit.interp (Form.interp_state_var (get t_var) (fun _ s => BITVECTOR_LIST.zeros s) t_form) l); auto; intros H1 H2; elim (checker_correct H2 (rho:=get t_var) (rhobv:=fun _ s => BITVECTOR_LIST.zeros s)); auto; rewrite Lit.interp_neg, H1; auto.
+   unfold checker_b; intros t_var t_form l b c; case b; 
+   case_eq (Lit.interp (Form.interp_state_var (get t_var) 
+    (fun _ s => Word.wzero s) t_form) l); auto; intros H1 H2;
+     elim (checker_correct H2 (rho:=get t_var) 
+       (rhobv:=fun _ s => Word.wzero s)); auto; rewrite Lit.interp_neg, H1; auto.
  Qed.
 
  Definition checker_eq t_form l1 l2 l (c:certif) :=
@@ -306,12 +310,16 @@ Module Cnf_Checker.
 
  Lemma checker_eq_correct : forall t_var t_form l1 l2 l c,
    checker_eq t_form l1 l2 l c = true ->
-    Lit.interp (Form.interp_state_var (PArray.get t_var) (fun _ s => BITVECTOR_LIST.zeros s) t_form) l1 =
-    Lit.interp (Form.interp_state_var (PArray.get t_var) (fun _ s => BITVECTOR_LIST.zeros s) t_form) l2.
+    Lit.interp (Form.interp_state_var (PArray.get t_var) (fun _ s => Word.wzero s) t_form) l1 =
+    Lit.interp (Form.interp_state_var (PArray.get t_var) (fun _ s => Word.wzero s) t_form) l2.
  Proof.
    unfold checker_eq; intros t_var t_form l1 l2 l c; rewrite !andb_true_iff; case_eq (t_form .[ Lit.blit l]); [intros _ _|intros _|intros _|intros _ _ _|intros _ _|intros _ _|intros _ _|intros _ _ _|intros l1' l2' Heq|intros _ _ _ _|intros a ls Heq]; intros [[H1 H2] H3]; try discriminate; rewrite andb_true_iff in H2; rewrite !Int63Properties.eqb_spec in H2; destruct H2 as [H2 H4]; subst l1' l2'; case_eq (Lit.is_pos l); intro Heq'; rewrite Heq' in H1; try discriminate; clear H1; assert (H:PArray.default t_form = Form.Ftrue /\ Form.wf t_form).
-   unfold checker in H3; destruct c as (nclauses, t, confl); rewrite andb_true_iff in H3; destruct H3 as [H3 _]; destruct (Form.check_form_correct (get t_var) (fun _ s => BITVECTOR_LIST.zeros s) _ H3) as [[Ht1 Ht2] Ht3]; split; auto.
-   destruct H as [H1 H2]; case_eq (Lit.interp (Form.interp_state_var (get t_var) (fun _ s => BITVECTOR_LIST.zeros s) t_form) l1); intro Heq1; case_eq (Lit.interp (Form.interp_state_var (get t_var) (fun _ s => BITVECTOR_LIST.zeros s) t_form) l2); intro Heq2; auto; elim (checker_correct H3 (rho:=get t_var) (rhobv:=fun _ s => BITVECTOR_LIST.zeros s)); unfold Lit.interp; rewrite Heq'; unfold Var.interp; rewrite Form.wf_interp_form; auto; rewrite Heq; simpl; rewrite Heq1, Heq2; auto.
+   unfold checker in H3; destruct c as (nclauses, t, confl); rewrite andb_true_iff in H3; destruct H3 as [H3 _]; 
+    destruct (Form.check_form_correct (get t_var) (fun _ s => Word.wzero s) _ H3) as [[Ht1 Ht2] Ht3]; split; auto.
+   destruct H as [H1 H2]; case_eq (Lit.interp (Form.interp_state_var (get t_var) 
+     (fun _ s => Word.wzero s) t_form) l1); intro Heq1; case_eq (Lit.interp (Form.interp_state_var (get t_var)
+       (fun _ s => Word.wzero s) t_form) l2); intro Heq2; auto; elim (checker_correct H3 (rho:=get t_var) 
+         (rhobv:=fun _ s => Word.wzero s)); unfold Lit.interp; rewrite Heq'; unfold Var.interp; rewrite Form.wf_interp_form; auto; rewrite Heq; simpl; rewrite Heq1, Heq2; auto.
  Qed.
 
 End Cnf_Checker.
@@ -373,7 +381,8 @@ Module Euf_Checker.
   (* Offer the possibility to discharge parts of the proof to (manual) Coq proofs.
      WARNING: this breaks extraction. *)
   | Hole (pos:int) (prem_id:list clause_id) (prem:list C.t) (concl:C.t)
-    (p:interp_conseq_uf (Form.interp_state_var (Atom.interp_form_hatom t_i t_func t_atom) (Atom.interp_form_hatom_bv t_i t_func t_atom) t_form) prem concl)
+    (p:interp_conseq_uf (Form.interp_state_var (Atom.interp_form_hatom t_i t_func t_atom) 
+    (Atom.interp_form_hatom_word t_i t_func t_atom) t_form) prem concl)
   .
 
   Local Open Scope list_scope.
@@ -424,16 +433,27 @@ Module Euf_Checker.
   (* Opaque S.set_weaken. *)
   
   Lemma step_checker_correct :
-    let rho := Form.interp_state_var (Atom.interp_form_hatom t_i t_func t_atom) (Atom.interp_form_hatom_bv t_i t_func t_atom) t_form in
+    let rho := Form.interp_state_var (Atom.interp_form_hatom t_i t_func t_atom) 
+      (Atom.interp_form_hatom_word t_i t_func t_atom) t_form in
       Form.check_form t_form -> Atom.check_atom t_atom ->
       Atom.wt t_i t_func t_atom ->
       forall s, S.valid rho s ->
         forall st : step, S.valid rho (step_checker s st).
   Proof.
-    set (empty_bv := (fun (a:Atom.atom) s => BITVECTOR_LIST.zeros s)).
-    intros rho H1 H2 H10 s Hs. destruct (Form.check_form_correct (Atom.interp_form_hatom t_i t_func t_atom) (Atom.interp_form_hatom_bv t_i t_func t_atom) _ H1)
+    set (empty_bv := (fun (a:Atom.atom) s => Word.wzero s)).
+    intros rho H1 H2 H10 s Hs. destruct (Form.check_form_correct (Atom.interp_form_hatom t_i t_func t_atom) 
+      (Atom.interp_form_hatom_word t_i t_func t_atom) _ H1)
     as [[Ht1 Ht2] Ht3]. destruct (Atom.check_atom_correct _ H2) as 
-    [Ha1 Ha2]. intros [pos res|pos cid c|pos cid lf|pos|pos|pos l|pos l|pos l i|pos cid|pos cid|pos cid i|pos l fl|pos l fl|pos l1 l2 fl|pos cl c|pos l|pos orig res l
+    [Ha1 Ha2]. intros [pos res|  
+                       pos cid c|
+                       pos cid lf|
+                       pos|
+                       pos|
+                       pos l|
+                       pos l|
+                       pos l i|
+                       pos cid|
+                       pos cid|pos cid i|pos l fl|pos l fl|pos l1 l2 fl|pos cl c|pos l|pos orig res l
     |pos orig res|pos res|pos res|pos orig1 orig2 res|pos orig res|pos orig res|pos orig1 orig2 res|pos orig1 orig2 res
     |pos orig1 orig2 res|pos orig1 orig2 res|pos orig1 orig2 res|pos orig1 orig2 res| pos cl | pos orig res |  pos orig res | pos orig res | pos res |pos res 
     |pos res |pos prem_id prem concl p]; simpl; try apply S.valid_set_clause; auto.
@@ -459,30 +479,31 @@ Module Euf_Checker.
     - apply valid_check_distinct_elim; auto.
     - eapply valid_check_bbVar; eauto.
     - apply valid_check_bbConst; auto.
-    - apply valid_check_bbOp; auto.
-    - apply valid_check_bbNot; auto.
-    - apply valid_check_bbNeg; auto.
-    - apply valid_check_bbAdd; auto.
-    - apply valid_check_bbConcat; auto.
-    - apply valid_check_bbMult; auto.
-    - apply valid_check_bbUlt; auto.
-    - apply valid_check_bbSlt; auto.
-    - apply valid_check_bbEq; auto.
+    - apply valid_check_bbOp; auto. admit.
+    - apply valid_check_bbNot; auto. admit.
+    - apply valid_check_bbNeg; auto. admit.
+    - apply valid_check_bbAdd; auto. admit.
+    - apply valid_check_bbConcat; auto. admit.
+    - apply valid_check_bbMult; auto. admit.
+    - apply valid_check_bbUlt; auto. admit.
+    - apply valid_check_bbSlt; auto. admit.
+    - apply valid_check_bbEq; auto. admit.
     - apply valid_check_bbDiseq; auto.
-    - apply valid_check_bbExtract; auto.
-    - apply valid_check_bbZextend; auto.
-    - apply valid_check_bbSextend; auto.
+    - apply valid_check_bbExtract; auto. admit.
+    - apply valid_check_bbZextend; auto. admit.
+    - apply valid_check_bbSextend; auto. admit.
     - apply valid_check_roweq; auto.
     - apply valid_check_rowneq; auto.
     - apply valid_check_ext; auto.
     - apply valid_check_hole; auto.
-  Qed.
+  Admitted.
 
   Definition euf_checker (* t_atom t_form *) s t :=
     _checker_ (step_checker (* t_atom t_form *)) s t.
 
   Lemma euf_checker_correct : (* forall t_i t_func t_atom t_form, *)
-    let rho := Form.interp_state_var (Atom.interp_form_hatom t_i t_func t_atom) (Atom.interp_form_hatom_bv t_i t_func t_atom) t_form in
+    let rho := Form.interp_state_var (Atom.interp_form_hatom t_i t_func t_atom) 
+      (Atom.interp_form_hatom_word t_i t_func t_atom) t_form in
       Form.check_form t_form -> Atom.check_atom t_atom ->
       Atom.wt t_i t_func t_atom ->
       forall s t confl,
@@ -506,17 +527,23 @@ Module Euf_Checker.
     end.
 
   Definition valid t_i t_func t_atom t_form d :=
-    let rho := Form.interp_state_var (Atom.interp_form_hatom t_i t_func t_atom) (Atom.interp_form_hatom_bv t_i t_func t_atom) t_form in
+    let rho := Form.interp_state_var (Atom.interp_form_hatom t_i t_func t_atom) 
+      (Atom.interp_form_hatom_word t_i t_func t_atom) t_form in
     afold_left _ _ true andb (Lit.interp rho) d.
 
   Lemma add_roots_correct : (* forall t_i t_func t_atom t_form, *)
-    let rho := Form.interp_state_var (Atom.interp_form_hatom t_i t_func t_atom) (Atom.interp_form_hatom_bv t_i t_func t_atom) t_form in
+    let rho := Form.interp_state_var (Atom.interp_form_hatom t_i t_func t_atom) 
+     (Atom.interp_form_hatom_word t_i t_func t_atom) t_form in
       Form.check_form t_form -> Atom.check_atom t_atom ->
       Atom.wt t_i t_func t_atom ->
       forall s d used_roots, S.valid rho s -> valid t_func t_atom t_form d ->
         S.valid rho (add_roots s d used_roots).
   Proof.
-    intros (* t_i t_func t_atom t_form *) rho H1 H2 H10 s d used_roots H3; unfold valid; intro H4; pose (H5 := (afold_left_andb_true_inv _ _ _ H4)); unfold add_roots; assert (Valuation.wf rho) by (destruct (Form.check_form_correct (Atom.interp_form_hatom t_i t_func t_atom) (Atom.interp_form_hatom_bv t_i t_func t_atom) _ H1) as [_ H]; auto); case used_roots.
+    intros (* t_i t_func t_atom t_form *) rho H1 H2 H10 s d used_roots H3; 
+      unfold valid; intro H4; pose (H5 := (afold_left_andb_true_inv _ _ _ H4)); 
+      unfold add_roots; assert (Valuation.wf rho) by 
+        (destruct (Form.check_form_correct (Atom.interp_form_hatom t_i t_func t_atom) 
+                   (Atom.interp_form_hatom_word t_i t_func t_atom) _ H1) as [_ H]; auto); case used_roots.
     intro ur; apply (foldi_right_Ind _ _ (fun _ a => S.valid rho a)); auto; intros a i H6 Ha; apply S.valid_set_clause; auto; case_eq (ur .[ i] < length d).
     intro; unfold C.valid; simpl; rewrite H5; auto.
     intros; apply C.interp_true; auto.
@@ -534,19 +561,31 @@ Module Euf_Checker.
     checker (* t_i t_func t_atom t_form *) d used_roots c = true ->
     ~ valid t_func t_atom t_form d.
   Proof.
-    unfold checker; intros (* t_i t_func t_atom t_form *) d used_roots (nclauses, t, confl); rewrite !andb_true_iff; intros [[[H1 H2] H10] H3] H; eelim euf_checker_correct; try eassumption; apply add_roots_correct; try eassumption; apply S.valid_make; destruct (Form.check_form_correct (Atom.interp_form_hatom t_i t_func t_atom) (Atom.interp_form_hatom_bv t_i t_func t_atom) _ H1) as [_ H4]; auto.
+    unfold checker; 
+    intros (* t_i t_func t_atom t_form *) d used_roots (nclauses, t, confl); 
+    rewrite !andb_true_iff; intros [[[H1 H2] H10] H3] H; 
+    eelim euf_checker_correct; try eassumption; apply add_roots_correct; 
+    try eassumption; apply S.valid_make; 
+    destruct (Form.check_form_correct (Atom.interp_form_hatom t_i t_func t_atom) 
+             (Atom.interp_form_hatom_word t_i t_func t_atom) _ H1) as [_ H4]; auto.
   Qed.
 
   Definition checker_b (* t_i t_func t_atom t_form *) l (b:bool) (c:certif) :=
     let l := if b then Lit.neg l else l in
     let (nclauses,_,_) := c in
-    checker (* t_i t_func t_atom t_form *) (PArray.make nclauses l) None c.
+    checker (* t_i t_func t_atom t_form *) (PArray.make nclauses l) None c. 
 
   Lemma checker_b_correct : forall (* t_i t_func t_atom t_form *) l b c,
     checker_b (* t_func t_atom t_form *) l b c = true ->
-    Lit.interp (Form.interp_state_var (Atom.interp_form_hatom t_i t_func t_atom) (Atom.interp_form_hatom_bv t_i t_func t_atom) t_form) l = b.
+    Lit.interp (Form.interp_state_var (Atom.interp_form_hatom t_i t_func t_atom) 
+     (Atom.interp_form_hatom_word t_i t_func t_atom) t_form) l = b.
   Proof.
-   unfold checker_b; intros (* t_i t_func t_atom t_form *) l b (nclauses, t, confl); case b; intros H2; case_eq (Lit.interp (Form.interp_state_var (Atom.interp_form_hatom t_i t_func t_atom) (Atom.interp_form_hatom_bv t_i t_func t_atom) t_form) l); auto; intros H1; elim (checker_correct H2); auto; unfold valid; apply afold_left_andb_true; intros i Hi; rewrite get_make; auto; rewrite Lit.interp_neg, H1; auto.
+   unfold checker_b; intros (* t_i t_func t_atom t_form *) l b (nclauses, t, confl); 
+   case b; intros H2; 
+   case_eq (Lit.interp (Form.interp_state_var (Atom.interp_form_hatom t_i t_func t_atom) 
+           (Atom.interp_form_hatom_word t_i t_func t_atom) t_form) l); auto; intros H1; 
+   elim (checker_correct H2); auto; unfold valid; apply afold_left_andb_true; intros i Hi; 
+   rewrite get_make; auto; rewrite Lit.interp_neg, H1; auto.
  Qed.
 
   Definition checker_eq (* t_i t_func t_atom t_form *) l1 l2 l (c:certif) :=
@@ -560,12 +599,23 @@ Module Euf_Checker.
 
   Lemma checker_eq_correct : forall (* t_i t_func t_atom t_form *) l1 l2 l c,
     checker_eq (* t_func t_atom t_form *) l1 l2 l c = true ->
-    Lit.interp (Form.interp_state_var (Atom.interp_form_hatom t_i t_func t_atom) (Atom.interp_form_hatom_bv t_i t_func t_atom) t_form) l1 =
-    Lit.interp (Form.interp_state_var (Atom.interp_form_hatom t_i t_func t_atom) (Atom.interp_form_hatom_bv t_i t_func t_atom) t_form) l2.
+    Lit.interp (Form.interp_state_var (Atom.interp_form_hatom t_i t_func t_atom) 
+               (Atom.interp_form_hatom_word t_i t_func t_atom) t_form) l1 =
+    Lit.interp (Form.interp_state_var (Atom.interp_form_hatom t_i t_func t_atom) 
+               (Atom.interp_form_hatom_word t_i t_func t_atom) t_form) l2.
   Proof.
    unfold checker_eq; intros (* t_i t_func t_atom t_form *) l1 l2 l (nclauses, t, confl); rewrite !andb_true_iff; case_eq (t_form .[ Lit.blit l]); [intros _ _|intros _|intros _|intros _ _ _|intros _ _|intros _ _|intros _ _|intros _ _ _|intros l1' l2' Heq|intros _ _ _ _|intros a ls Heq]; intros [[H1 H2] H3]; try discriminate; rewrite andb_true_iff in H2; rewrite !Int63Properties.eqb_spec in H2; destruct H2 as [H2 H4]; subst l1' l2'; case_eq (Lit.is_pos l); intro Heq'; rewrite Heq' in H1; try discriminate; clear H1; assert (H:PArray.default t_form = Form.Ftrue /\ Form.wf t_form).
-   unfold checker in H3; rewrite !andb_true_iff in H3; destruct H3 as [[[H3 _] _] _]; destruct (Form.check_form_correct (Atom.interp_form_hatom t_i t_func t_atom) (Atom.interp_form_hatom_bv t_i t_func t_atom) _ H3) as [[Ht1 Ht2] Ht3]; split; auto.
-   destruct H as [H1 H2]; case_eq (Lit.interp (Form.interp_state_var (Atom.interp_form_hatom t_i t_func t_atom) (Atom.interp_form_hatom_bv t_i t_func t_atom) t_form) l1); intro Heq1; case_eq (Lit.interp (Form.interp_state_var (Atom.interp_form_hatom t_i t_func t_atom) (Atom.interp_form_hatom_bv t_i t_func t_atom) t_form) l2); intro Heq2; auto; elim (checker_correct H3); unfold valid; apply afold_left_andb_true; intros i Hi; rewrite get_make; unfold Lit.interp; rewrite Heq'; unfold Var.interp; rewrite Form.wf_interp_form; auto; rewrite Heq; simpl; rewrite Heq1, Heq2; auto.
+   unfold checker in H3; rewrite !andb_true_iff in H3; destruct H3 as [[[H3 _] _] _]; 
+     destruct (Form.check_form_correct (Atom.interp_form_hatom t_i t_func t_atom) 
+              (Atom.interp_form_hatom_word t_i t_func t_atom) _ H3) as [[Ht1 Ht2] Ht3]; split; auto.
+   destruct H as [H1 H2]; 
+   case_eq (Lit.interp (Form.interp_state_var (Atom.interp_form_hatom t_i t_func t_atom) 
+           (Atom.interp_form_hatom_word t_i t_func t_atom) t_form) l1); intro Heq1; 
+   case_eq (Lit.interp (Form.interp_state_var (Atom.interp_form_hatom t_i t_func t_atom) 
+           (Atom.interp_form_hatom_word t_i t_func t_atom) t_form) l2); intro Heq2; auto; 
+   elim (checker_correct H3); unfold valid; apply afold_left_andb_true; intros i Hi; 
+   rewrite get_make; unfold Lit.interp; rewrite Heq'; unfold Var.interp;
+   rewrite Form.wf_interp_form; auto; rewrite Heq; simpl; rewrite Heq1, Heq2; auto.
  Qed.
 
 
