src/array/Array_checker.v
@@ -156,11 +156,11 @@ Section certif.
     Local Notation interp_form_hatom :=
       (Atom.interp_form_hatom t_i t_func t_atom).
 
-    Local Notation interp_form_hatom_bv :=
-      (Atom.interp_form_hatom_bv t_i t_func t_atom).
+    Local Notation interp_form_hatom_word :=
+      (Atom.interp_form_hatom_word t_i t_func t_atom).
 
     Local Notation rho :=
-      (Form.interp_state_var interp_form_hatom interp_form_hatom_bv t_form).
+      (Form.interp_state_var interp_form_hatom interp_form_hatom_word t_form).
 
     Local Notation t_interp := (t_interp t_i t_func t_atom).
 
@@ -175,31 +175,33 @@ Section certif.
     Let def_t_form : default t_form = Form.Ftrue.
     Proof.
       destruct (Form.check_form_correct
-                  interp_form_hatom interp_form_hatom_bv _ ch_form) as [H _];
+                  interp_form_hatom interp_form_hatom_word _ ch_form) as [H _];
         destruct H; auto.
     Qed.
 
     Let wf_t_form : Form.wf t_form.
     Proof.
       destruct (Form.check_form_correct
-                  interp_form_hatom interp_form_hatom_bv _ ch_form) as [H _];
+                  interp_form_hatom interp_form_hatom_word _ ch_form) as [H _];
         destruct H; auto.
     Qed.
 
     Let wf_rho : Valuation.wf rho.
     Proof.
       destruct (Form.check_form_correct
-                  interp_form_hatom interp_form_hatom_bv _ ch_form); auto.
+                  interp_form_hatom interp_form_hatom_word _ ch_form); auto.
     Qed.
 
     Let rho_interp : forall x : int,
-        rho x = Form.interp interp_form_hatom interp_form_hatom_bv t_form (t_form.[ x]).
+        rho x = Form.interp interp_form_hatom interp_form_hatom_word t_form (t_form.[ x]).
     Proof. intros x;apply wf_interp_form;trivial. Qed.
 
     Definition wf := PArray.forallbi lt_form t_form.
 
     Hypothesis wf_t_i : wf.
     Notation atom := int (only parsing).
+
+
 
     
     Lemma valid_check_roweq lres : C.valid rho (check_roweq lres).
@@ -209,9 +211,9 @@ Section certif.
       case_eq (t_form .[ Lit.blit lres]); try (intros; now apply C.interp_true).
       intros a Heq2.
       case_eq (t_atom .[ a]); try (intros; now apply C.interp_true).
-      intros [ | | | | | | | |N|N|N|N|N|N|N|N|N| | ] a1 a2 Heq3; try (intros; now apply C.interp_true).
+      intros [ | | | | | | | |N|N|N|N|N|N|N|N| | ] a1 a2 Heq3; try (intros; now apply C.interp_true).
       case_eq (t_atom .[ a1]); try (intros; now apply C.interp_true).
-      intros [ | | | | | | | |N|N|N|N|N|N|N|N|N| | ] b1 b2 Heq4; try (intros; now apply C.interp_true).
+      intros [ | | | | | | | |N|N|N|N|N|N|N|N| | ] b1 b2 Heq4; try (intros; now apply C.interp_true).
       case_eq (t_atom .[ b1]); try (intros; now apply C.interp_true).
       intros [ ] c1 c2 c3 Heq5.
       (* roweq *)
@@ -405,8 +407,6 @@ Section certif.
         exact (Typ.dec_interp _ _).
     Qed.
 
-
-    
     Lemma valid_check_rowneq cl : C.valid rho (check_rowneq cl).
     Proof.
         unfold check_rowneq.
@@ -420,13 +420,13 @@ Section certif.
         case_eq (t_form .[ Lit.blit j]); try (intros; now apply C.interp_true).
         intros b Heq4.
         case_eq (t_atom .[ a]); try (intros; now apply C.interp_true).
-        intros [ | | | | | | | |N|N|N|N|N|N|N|N|N| | ] a1 a2 Heq5; try (intros; now apply C.interp_true).
+        intros [ | | | | | | | |N|N|N|N|N|N|N|N| | ] a1 a2 Heq5; try (intros; now apply C.interp_true).
         case_eq (t_atom .[ b]); try (intros; now apply C.interp_true).
-        intros [ | | | | | | | |N|N|N|N|N|N|N|N|N| | ] b1 b2 Heq6; try (intros; now apply C.interp_true).
+        intros [ | | | | | | | |N|N|N|N|N|N|N|N| | ] b1 b2 Heq6; try (intros; now apply C.interp_true).
         case_eq (t_atom .[ b1]); try (intros; now apply C.interp_true).
-        intros [ | | | | | | | |N|N|N|N|N|N|N|N|N| | ] c1 c2 Heq7; try (intros; now apply C.interp_true).
+        intros [ | | | | | | | |N|N|N|N|N|N|N|N| | ] c1 c2 Heq7; try (intros; now apply C.interp_true).
         case_eq (t_atom .[ b2]); try (intros; now apply C.interp_true).
-        intros [ | | | | | | | |N|N|N|N|N|N|N|N|N| | ] d1 d2 Heq8; try (intros; now apply C.interp_true).
+        intros [ | | | | | | | |N|N|N|N|N|N|N|N| | ] d1 d2 Heq8; try (intros; now apply C.interp_true).
         case_eq (Typ.eqb t t1 && Typ.eqb t t3 && Typ.eqb t0 t2 && Typ.eqb t0 t4); 
           try (intros; now apply C.interp_true). intros Heq9.
 
@@ -899,8 +899,6 @@ Section certif.
     Qed.
 
 
-    
-    
   Axiom afold_left_or : forall a,
     afold_left bool int false orb (Lit.interp rho) a =
     C.interp rho (to_list a).
@@ -920,20 +918,20 @@ Require Import Psatz.
       case_eq (t_form .[ Lit.blit (a .[1])]); try (intros; now apply C.interp_true).
       intros c Heq6.
       case_eq (t_atom .[ b]); try (intros; now apply C.interp_true).
-      intros [ | | | | | | | |N|N|N|N|N|N|N|N|N| | ] b1 b2 Heq7; try (intros; now apply C.interp_true).
+      intros [ | | | | | | | |N|N|N|N|N|N|N|N| | ] b1 b2 Heq7; try (intros; now apply C.interp_true).
       case_eq t; try (intros; now apply C.interp_true). intros t0 t1 Heq8.
       case_eq (t_atom .[ c]); try (intros; now apply C.interp_true).
-      intros [ | | | | | | | |N|N|N|N|N|N|N|N|N| | ] c1 c2 Heq9; try (intros; now apply C.interp_true).
+      intros [ | | | | | | | |N|N|N|N|N|N|N|N| | ] c1 c2 Heq9; try (intros; now apply C.interp_true).
       case_eq (Typ.eqb t1 t2); [ intros Heq10 | intros Heq10; now apply C.interp_true].
       case_eq (t_atom .[ c1]); try (intros; now apply C.interp_true).
-      intros [ | | | | | | | |N|N|N|N|N|N|N|N|N| | ] d1 d2 Heq11; try (intros; now apply C.interp_true).
+      intros [ | | | | | | | |N|N|N|N|N|N|N|N| | ] d1 d2 Heq11; try (intros; now apply C.interp_true).
       case_eq (t_atom .[ c2]); try (intros; now apply C.interp_true).
-      intros [ | | | | | | | |N|N|N|N|N|N|N|N|N| | ] e1 e2 Heq12; try (intros; now apply C.interp_true).
+      intros [ | | | | | | | |N|N|N|N|N|N|N|N| | ] e1 e2 Heq12; try (intros; now apply C.interp_true).
       case_eq (Typ.eqb t0 t3 && Typ.eqb t0 t5 && Typ.eqb t1 t4 && Typ.eqb t1 t6 && 
                   (b1 == d1) && (b2 == e1) && (d2 == e2)); 
                   [ intros Heq13 | intros Heq13; now apply C.interp_true].
       case_eq (t_atom .[ d2]); try (intros; now apply C.interp_true).
-      intros [ | | | | | | | |N|N|N|N|N|N|N|N|N| | ] f1 f2 Heq14; try (intros; now apply C.interp_true).
+      intros [ | | | | | | | |N|N|N|N|N|N|N|N| | ] f1 f2 Heq14; try (intros; now apply C.interp_true).
 
       case_eq (Typ.eqb t0 t7 && Typ.eqb t1 t8 && (f1 == b1) && (f2 == b2)); 
                 [ intros Heq15 | intros Heq15; now apply C.interp_true].
